WIP

mem/OpenDef.v
@@ -20,575 +20,31 @@ Set Implicit Arguments.
 Section AUX.
   Context `{Σ: GRA.t}.
   Definition fspec_trivial: fspec :=
-    mk_fspec (meta:=unit) (fun _ argh argl o => (⌜argh = argl ∧ o = ord_top⌝: iProp)%I)
-             (fun _ reth retl => (⌜reth = retl⌝: iProp)%I)
+    mk_fspec (meta:=unit) (fun _ _ argh argl o => (⌜argh = argl ∧ o = ord_top⌝: iProp)%I)
+             (fun _ _ reth retl => (⌜reth = retl⌝: iProp)%I)
   .
 
 End AUX.
+
 
 
 (*** TODO: remove redundancy ***)
 Ltac my_red_both := try (prw _red_gen 2 0); try (prw _red_gen 1 0).
 
-
-
-(******************************************* UNKNOWN ***********************************************)
-(******************************************* UNKNOWN ***********************************************)
-(******************************************* UNKNOWN ***********************************************)
-Section AUX.
-  Variant uCallE: Type -> Type :=
-  | uCall (fn: gname) {X} (args: X): uCallE Any.t
-  .
-  Constraint uCallE.u1 < Any.t.u0.
-End AUX.
-
-Module UModSem.
-Section UMODSEM.
-
-  Context `{Σ: GRA.t}.
-
-  Record t: Type := mk {
-    fnsems: list (gname * (Any.t -> itree (uCallE +' pE +' eventE) Any.t));
-    mn: mname;
-    initial_st: Any.t;
-  }
-  .
-
-  (************************* MOD ***************************)
-  (************************* MOD ***************************)
-  (************************* MOD ***************************)
-
-  Definition transl_uCallE: uCallE ~> callE :=
-    fun T '(uCall fn args) => Call fn args↑
-  .
-
-  Definition transl_event: (uCallE +' pE +' eventE) ~> (callE +' pE +' eventE) :=
-    (bimap transl_uCallE (bimap (id_ _) (id_ _)))
-  .
-
-  Definition transl_itr: itree (uCallE +' pE +' eventE) ~> itree Es :=
-    fun _ itr => resum_itr (E:=callE +' pE +' eventE) (F:=Es)
-                           (interp (T:=_) (fun _ e => trigger (transl_event e)) itr)
-  .
-
-  Definition transl_fun: (Any.t -> itree (uCallE +' pE +' eventE) Any.t) -> (Any.t -> itree Es Any.t) :=
-    fun ktr => (transl_itr (T:=_) ∘ ktr)
-  .
-
-  Definition transl (ms: t): ModSem.t := {|
-    (* ModSem.fnsems := List.map (map_snd (((∘)∘(∘)) (resum_itr (T:=Any.t)) cfun)) ms.(fnsems); *)
-    ModSem.fnsems := List.map (map_snd transl_fun) ms.(fnsems);
-    ModSem.mn := ms.(mn);
-    ModSem.initial_mr := ε;
-    ModSem.initial_st := ms.(initial_st);
-  |}
-  .
-
-  (*****************************************************)
-  (****************** Reduction Lemmas *****************)
-  (*****************************************************)
-
-  Lemma transl_itr_bind
-        (R S: Type)
-        (s: itree (uCallE +' pE +' eventE) R) (k : R -> itree (uCallE +' pE +' eventE) S)
-    :
-      (transl_itr (s >>= k))
-      =
-      ((transl_itr s) >>= (fun r => transl_itr (k r))).
-  Proof.
-    unfold transl_itr in *. grind. my_red_both. grind.
-  Qed.
-
-  Lemma transl_itr_tau
-        (U: Type)
-        (t : itree _ U)
-    :
-      (transl_itr (Tau t))
-      =
-      (Tau (transl_itr t)).
-  Proof.
-    unfold transl_itr in *. grind. my_red_both. grind.
-  Qed.
-
-  Lemma transl_itr_ret
-        (U: Type)
-        (t: U)
-    :
-      ((transl_itr (Ret t)))
-      =
-      Ret t.
-  Proof.
-    unfold transl_itr in *. grind. my_red_both. grind.
-  Qed.
-
-  Lemma transl_itr_triggerp
-        (R: Type)
-        (i: pE R)
-    :
-      (transl_itr (trigger i))
-      =
-      (trigger i >>= (fun r => tau;; tau;; Ret r)).
-  Proof.
-    unfold transl_itr in *.
-    repeat rewrite interp_trigger. repeat (my_red_both; grind; resub).
-  Qed.
-
-  Lemma transl_itr_triggere
-        (R: Type)
-        (i: eventE R)
-    :
-      (transl_itr (trigger i))
-      =
-      (trigger i >>= (fun r => tau;; tau;; Ret r)).
-  Proof.
-    unfold transl_itr in *.
-    repeat rewrite interp_trigger. repeat (my_red_both; grind; resub).
-  Qed.
-
-  Lemma transl_itr_ucall
-        (R: Type)
-        (i: uCallE R)
-    :
-      (transl_itr (trigger i))
-      =
-      (trigger (transl_uCallE i) >>= (fun r => tau;; tau;; Ret r)).
-  Proof.
-    unfold transl_itr in *.
-    repeat rewrite interp_trigger. repeat (my_red_both; grind; resub).
-  Qed.
-
-  Lemma transl_itr_triggerUB
-        (R: Type)
-    :
-      (transl_itr (triggerUB))
-      =
-      triggerUB (A:=R).
-  Proof.
-    unfold transl_itr, triggerUB in *. rewrite unfold_interp. cbn. repeat (my_red_both; grind; resub).
-  Qed.
-
-  Lemma transl_itr_triggerNB
-        (R: Type)
-    :
-      (transl_itr (triggerNB))
-      =
-      triggerNB (A:=R).
-  Proof.
-    unfold transl_itr, triggerNB in *. rewrite unfold_interp. cbn. repeat (my_red_both; grind; resub).
-  Qed.
-
-  Lemma transl_itr_unwrapU
-        (R: Type)
-        (i: option R)
-    :
-      (transl_itr (unwrapU i))
-      =
-      (unwrapU i).
-  Proof.
-    unfold transl_itr, unwrapU in *. des_ifs.
-    { etrans.
-      { eapply transl_itr_ret. }
-      { grind. }
-    }
-    { etrans.
-      { eapply transl_itr_triggerUB. }
-      { unfold triggerUB. grind. }
-    }
-  Qed.
-
-  Lemma transl_itr_unwrapN
-        (R: Type)
-        (i: option R)
-    :
-      (transl_itr (unwrapN i))
-      =
-      (unwrapN i).
-  Proof.
-    unfold transl_itr, unwrapN in *. des_ifs.
-    { etrans.
-      { eapply transl_itr_ret. }
-      { grind. }
-    }
-    { etrans.
-      { eapply transl_itr_triggerNB. }
-      { unfold triggerNB. grind. }
-    }
-  Qed.
-
-  Lemma transl_itr_assume
-        P
-    :
-      (transl_itr (assume P))
-      =
-      (assume P;;; tau;; tau;; Ret tt)
-  .
-  Proof.
-    unfold assume. rewrite transl_itr_bind. rewrite transl_itr_triggere.
-    repeat (my_red_both; grind; resub).
-    eapply transl_itr_ret.
-  Qed.
-
-  Lemma transl_itr_guarantee
-        P
-    :
-      (transl_itr (guarantee P))
-      =
-      (guarantee P;;; tau;; tau;; Ret tt).
-  Proof.
-    unfold guarantee. rewrite transl_itr_bind. rewrite transl_itr_triggere.
-    repeat (my_red_both; grind; resub).
-    eapply transl_itr_ret.
-  Qed.
-
-  Lemma transl_itr_ext
-        R (itr0 itr1: itree _ R)
-        (EQ: itr0 = itr1)
-    :
-      (transl_itr itr0)
-      =
-      (transl_itr itr1)
-  .
-  Proof. subst; et. Qed.
-
-
-
-
-
-
-
-
-
-
-
-
-  (************************* SMOD ***************************)
-  (************************* SMOD ***************************)
-  (************************* SMOD ***************************)
-
-  Variable stb: (list (string * fspec)).
-
-  Definition massage_uCallE: uCallE ~> itree (hCallE +' pE +' eventE) :=
-    fun T '(uCall fn args) => _ <- (alist_find fn stb)?;; trigger (hCall false fn (args↑))
-  .
-
-  (* Definition massage_event: (uCallE +' pE +' eventE) ~> itree (hCallE +' pE +' eventE) := *)
-  (*   (case_ (bif:=sum1) (massage_uCallE) *)
-  (*          ((fun T X => trigger X): _ ~> itree (hCallE +' pE +' eventE))) *)
-  (* . *)
-
-  Definition massage_itr: itree (uCallE +' pE +' eventE) ~> itree (hCallE +' pE +' eventE) :=
-    interp (case_ (bif:=sum1) (massage_uCallE)
-                  ((fun T X => trigger X): _ ~> itree (hCallE +' pE +' eventE)))
-  .
-
-  Definition massage_fun (ktr: Any.t -> itree (uCallE +' pE +' eventE) Any.t):
-    (Any.t -> itree (hCallE +' pE +' eventE) Any.t) :=
-    (massage_itr (T:=_) ∘ ktr)
-  .
-
-  Definition massage_fsb: (Any.t -> itree (uCallE +' pE +' eventE) Any.t) -> fspecbody :=
-    fun ktr => mk_specbody fspec_trivial (massage_fun ktr)
-  .
-
-  Definition massage (ms: t): SModSem.t := {|
-    SModSem.fnsems := List.map (map_snd massage_fsb) ms.(fnsems);
-    SModSem.mn := ms.(mn);
-    SModSem.initial_mr := ε;
-    SModSem.initial_st := ms.(initial_st);
-  |}
-  .
-
-  (*****************************************************)
-  (****************** Reduction Lemmas *****************)
-  (*****************************************************)
-
-  Lemma massage_itr_bind
-        (R S: Type)
-        (s: itree (uCallE +' pE +' eventE) R) (k : R -> itree (uCallE +' pE +' eventE) S)
-    :
-      (massage_itr (s >>= k))
-      =
-      ((massage_itr s) >>= (fun r => massage_itr (k r))).
-  Proof.
-    unfold massage_itr in *. grind.
-  Qed.
-
-  Lemma massage_itr_tau
-        (U: Type)
-        (t : itree _ U)
-    :
-      (massage_itr (Tau t))
-      =
-      (Tau (massage_itr t)).
-  Proof.
-    unfold massage_itr in *. grind.
-  Qed.
-
-  Lemma massage_itr_ret
-        (U: Type)
-        (t: U)
-    :
-      ((massage_itr (Ret t)))
-      =
-      Ret t.
-  Proof.
-    unfold massage_itr in *. grind.
-  Qed.
-
-  Lemma massage_itr_triggerp
-        (R: Type)
-        (i: pE R)
-    :
-      (massage_itr (trigger i))
-      =
-      (trigger i >>= (fun r => tau;; Ret r)).
-  Proof.
-    unfold massage_itr in *.
-    repeat rewrite interp_trigger. grind.
-  Qed.
-
-  Lemma massage_itr_triggere
-        (R: Type)
-        (i: eventE R)
-    :
-      (massage_itr (trigger i))
-      =
-      (trigger i >>= (fun r => tau;; Ret r)).
-  Proof.
-    unfold massage_itr in *.
-    repeat rewrite interp_trigger. grind.
-  Qed.
-
-  Lemma massage_itr_ucall
-        (R: Type)
-        (i: uCallE R)
-    :
-      (massage_itr (trigger i))
-      =
-      massage_uCallE i >>= (fun r => tau;; Ret r).
-  Proof.
-    unfold massage_itr in *.
-    repeat rewrite interp_trigger. grind.
-  Qed.
-
-  Lemma massage_itr_triggerUB
-        (R: Type)
-    :
-      (massage_itr (triggerUB))
-      =
-      triggerUB (A:=R).
-  Proof.
-    unfold massage_itr, triggerUB in *. rewrite unfold_interp. cbn. grind.
-  Qed.
-
-  Lemma massage_itr_triggerNB
-        (R: Type)
-    :
-      (massage_itr (triggerNB))
-      =
-      triggerNB (A:=R).
-  Proof.
-    unfold massage_itr, triggerNB in *. rewrite unfold_interp. cbn. grind.
-  Qed.
-
-  Lemma massage_itr_unwrapU
-        (R: Type)
-        (i: option R)
-    :
-      (massage_itr (unwrapU i))
-      =
-      (unwrapU i).
-  Proof.
-    unfold massage_itr, unwrapU in *. des_ifs.
-    { etrans.
-      { eapply massage_itr_ret. }
-      { grind. }
-    }
-    { etrans.
-      { eapply massage_itr_triggerUB. }
-      { unfold triggerUB. grind. }
-    }
-  Qed.
-
-  Lemma massage_itr_unwrapN
-        (R: Type)
-        (i: option R)
-    :
-      (massage_itr (unwrapN i))
-      =
-      (unwrapN i).
-  Proof.
-    unfold massage_itr, unwrapN in *. des_ifs.
-    { etrans.
-      { eapply massage_itr_ret. }
-      { grind. }
-    }
-    { etrans.
-      { eapply massage_itr_triggerNB. }
-      { unfold triggerNB. grind. }
-    }
-  Qed.
-
-  Lemma massage_itr_assume
-        P
-    :
-      (massage_itr (assume P))
-      =
-      (assume P;;; tau;; Ret tt)
-  .
-  Proof.
-    unfold assume. rewrite massage_itr_bind. rewrite massage_itr_triggere. grind. eapply massage_itr_ret.
-  Qed.
-
-  Lemma massage_itr_guarantee
-        P
-    :
-      (massage_itr (guarantee P))
-      =
-      (guarantee P;;; tau;; Ret tt).
-  Proof.
-    unfold guarantee. rewrite massage_itr_bind. rewrite massage_itr_triggere. grind. eapply massage_itr_ret.
-  Qed.
-
-  Lemma massage_itr_ext
-        R (itr0 itr1: itree _ R)
-        (EQ: itr0 = itr1)
-    :
-      (massage_itr itr0)
-      =
-      (massage_itr itr1)
-  .
-  Proof. subst; et. Qed.
-
-End UMODSEM.
-End UModSem.
-
-Coercion UModSem.transl: UModSem.t >-> ModSem.t.
-Coercion UModSem.massage: UModSem.t >-> SModSem.t.
-
-Section RDB.
-  Context `{Σ: GRA.t}.
-
-  Global Program Instance utransl_itr_rdb: red_database (mk_box (@UModSem.transl_itr)) :=
-    mk_rdb
-      0
-      (mk_box UModSem.transl_itr_bind)
-      (mk_box UModSem.transl_itr_tau)
-      (mk_box UModSem.transl_itr_ret)
-      (mk_box UModSem.transl_itr_ucall)
-      (mk_box UModSem.transl_itr_triggere)
-      (mk_box UModSem.transl_itr_triggerp)
-      (mk_box True)
-      (mk_box UModSem.transl_itr_triggerUB)
-      (mk_box UModSem.transl_itr_triggerNB)
-      (mk_box UModSem.transl_itr_unwrapU)
-      (mk_box UModSem.transl_itr_unwrapN)
-      (mk_box UModSem.transl_itr_assume)
-      (mk_box UModSem.transl_itr_guarantee)
-      (mk_box UModSem.transl_itr_ext)
-  .
-
-  Global Program Instance umassage_itr_rdb: red_database (mk_box (@UModSem.massage_itr)) :=
-    mk_rdb
-      0
-      (mk_box UModSem.massage_itr_bind)
-      (mk_box UModSem.massage_itr_tau)
-      (mk_box UModSem.massage_itr_ret)
-      (mk_box UModSem.massage_itr_ucall)
-      (mk_box UModSem.massage_itr_triggere)
-      (mk_box UModSem.massage_itr_triggerp)
-      (mk_box True)
-      (mk_box UModSem.massage_itr_triggerUB)
-      (mk_box UModSem.massage_itr_triggerNB)
-      (mk_box UModSem.massage_itr_unwrapU)
-      (mk_box UModSem.massage_itr_unwrapN)
-      (mk_box UModSem.massage_itr_assume)
-      (mk_box UModSem.massage_itr_guarantee)
-      (mk_box UModSem.massage_itr_ext)
-  .
-End RDB.
-
-
-
-
-Module UMod.
-Section UMOD.
-
-  Context `{Σ: GRA.t}.
-
-  Record t: Type := mk {
-    get_modsem: Sk.t -> UModSem.t;
-    sk: Sk.t;
-  }
-  .
-
-  Definition transl (md: t): Mod.t := {|
-    Mod.get_modsem := UModSem.transl ∘ md.(get_modsem);
-    Mod.sk := md.(sk);
-  |}
-  .
-
-  Lemma transl_comm: forall md skenv, UModSem.transl (md.(get_modsem) skenv) = (transl md).(Mod.get_modsem) skenv.
-  Proof. i. refl. Qed.
-
-
-  Definition massage (stb: Sk.t -> list (gname * fspec)) (md: t): SMod.t := {|
-    SMod.get_modsem := (fun sk => (UModSem.massage (stb sk) (md.(get_modsem) sk)));
-    SMod.sk := md.(sk);
-  |}
-  .
-
-  (* Lemma to_smod_comm: forall stb md skenv, UModSem.massage stb (md.(get_modsem) skenv) = (massage stb md).(SMod.get_modsem) skenv. *)
-  (* Proof. i. refl. Qed. *)
-
-End UMOD.
-End UMod.
-
-Coercion UMod.transl: UMod.t >-> Mod.t.
-Coercion UMod.massage: UMod.t >-> SMod.t.
-
-
-
-
-
-
-
-
-
-
-
-
-
-
-
-
-
-
+(*** TODO: move to TODOYJ ***)
+Definition my_if X (b: bool) (x0 x1: X): X := if b then x0 else x1.
+Lemma my_if_same: forall X b (x: X), my_if b x x = x. i. destruct b; ss. Qed.
 
 
 
 (********************************************* KNOWN ***********************************************)
 (********************************************* KNOWN ***********************************************)
 (********************************************* KNOWN ***********************************************)
-
-  (* Definition disclose_smodsem (ms: SModSem.t): SModSem.t := {| *)
-  (*   SModSem.fnsems     := List.map (map_snd disclose_fsb) ms.(SModSem.fnsems); *)
-  (*   SModSem.mn         := ms.(SModSem.mn); *)
-  (*   SModSem.initial_mr := ms.(SModSem.initial_mr); *)
-  (*   SModSem.initial_st := ms.(SModSem.initial_st); *)
-  (* |} *)
-  (* . *)
-
-  (* Definition disclose_smod (ms: SMod.t): SMod.t := {| *)
-  (*   SMod.get_modsem := disclose_smodsem ∘ ms.(SMod.get_modsem); *)
-  (*   SMod.sk := ms.(SMod.sk); *)
-  (* |} *)
-  (* . *)
 
 Section AUX.
   Context `{Σ: GRA.t}.
 
-  Variant kflag: Type := (** known and **) pure | (** known and **) impure | unknown.
+  Variant kflag: Type := (** known and **) pure | (** known and **) impure.
 
   Variant kCallE: Type -> Type :=
   | kCall (kf: kflag) (fn: gname) (varg: Any.t): kCallE Any.t
@@ -596,26 +52,14 @@ Section AUX.
 
   Record kspecbody := mk_kspecbody {
     ksb_fspec:> fspec;                                            (*** K -> K ***)
-    ksb_ubody: Any.t -> itree (kCallE +' pE +' eventE) Any.t;     (*** U -> K ***)
-    ksb_kbody: Any.t -> itree (kCallE +' pE +' eventE) Any.t;     (*** K -> K ***)
+    ksb_ubody: (mname * Any.t) -> itree (kCallE +' pE +' eventE) Any.t;     (*** U -> K ***)
+    ksb_kbody: (mname * Any.t) -> itree (kCallE +' pE +' eventE) Any.t;     (*** K -> K ***)
   }
   .
 
-  Definition ksb_trivial (body: Any.t -> itree (kCallE +' pE +' eventE) Any.t): kspecbody :=
+  Definition ksb_trivial (body: (mname * Any.t) -> itree (kCallE +' pE +' eventE) Any.t): kspecbody :=
     mk_kspecbody fspec_trivial body body
   .
-
-  Section AUX.
-    Context `{HasEventE: eventE -< E}.
-    Definition cfun2 X Y (f: X -> itree Es Y): Any.t -> itree Es Any.t :=
-      fun args => map_or_else (Any.split args)
-                              (fun '(_, args) => args <- unwrapN args↓;; ret <- f args;; Ret (ret↑))
-                              (args <- unwrapN args↓;; ret <- f args;; Ret (ret↑))
-    .
-    Context `{HaskCallE: kCallE -< E}.
-    Definition ckcall {X Y} (kf: kflag) (fn: gname) (varg: X): itree E Y :=
-      vret <- trigger (kCall kf fn varg↑);; vret <- vret↓ǃ;; Ret vret.
-  End AUX.
 
   Program Fixpoint _APCK (at_most: Ord.t) {wf Ord.lt at_most}: itree (kCallE +' pE +' eventE) unit :=
     break <- trigger (Choose _);;
@@ -666,16 +110,6 @@ Section KMODSEM.
 
   Context `{Σ: GRA.t}.
 
-  (*** K -> K: unit; tbr == true ***)
-  (*** K -> U: list val; tbr == false ***)
-  (**** TODO: maybe "val" is more appropriate return type??? Check this later ****)
-  (**** TODO: maybe "val" is more appropriate return type??? Check this later ****)
-  (**** TODO: maybe "val" is more appropriate return type??? Check this later ****)
-  (**** TODO: maybe "val" is more appropriate return type??? Check this later ****)
-  (**** TODO: maybe "val" is more appropriate return type??? Check this later ****)
-  (**** TODO: maybe "val" is more appropriate return type??? Check this later ****)
-  (**** TODO: maybe "val" is more appropriate return type??? Check this later ****)
-
   Record t: Type := mk {
     (* fnsems: list (gname * (list val -> itree (oCallE +' pE +' eventE) val)); *)
     fnsems: list (gname * kspecbody);
@@ -692,9 +126,8 @@ Section KMODSEM.
   Definition transl_kCallE: kCallE ~> hCallE :=
     fun _ '(kCall kf fn args) =>
       match kf with
-      | pure => hCall true fn (Any.pair tt↑ args)
-      | impure => hCall false fn (Any.pair tt↑ args)
-      | unknown => hCall false fn args
+      | pure => hCall true fn args
+      | impure => hCall false fn args
       end
   .
 
@@ -706,28 +139,30 @@ Section KMODSEM.
     fun _ => interp (T:=_) (fun _ e => trigger (transl_event e))
   .
 
-  Definition transl_fun (ktr: Any.t -> itree (kCallE +' pE +' eventE) Any.t):
-    Any.t -> itree (hCallE +' pE +' eventE) Any.t :=
+  Definition transl_fun (ktr: (mname * Any.t) -> itree (kCallE +' pE +' eventE) Any.t):
+    (mname * Any.t) -> itree (hCallE +' pE +' eventE) Any.t :=
     (transl_itr (T:=_)) ∘ ktr
   .
 
+  Variable (frds: list mname).
+
   Definition disclose (fs: fspec): fspec :=
     mk_fspec (meta:=option fs.(meta))
-             (fun ox argh argl o =>
-                match ox, Any.split argh with
-                | Some x, Some (_, argh) => (fs.(precond) x argh argl o)
-                | None, None => ((⌜argh = argl /\ o = ord_top⌝): iProp)%I
-                | _, _ => (⌜False⌝: iProp)%I
+             (fun mn ox argh argl o =>
+                match ox with
+                | Some x => ((⌜In mn frds⌝: iProp) ∧ (fs.(precond) mn x argh argl o))%I
+                | None => ((⌜~(In mn frds) /\ argh = argl /\ o = ord_top⌝): iProp)%I
                 end)
-             (fun ox reth retl =>
-                map_or_else ox (fun x => (fs.(postcond) x reth retl)) (⌜reth = retl⌝: iProp)%I)
+             (fun mn ox reth retl =>
+                map_or_else ox (fun x => (fs.(postcond) mn x reth retl)) (⌜reth = retl⌝: iProp)%I)
   .
 
   Definition disclose_ksb (ksb: kspecbody): fspecbody :=
     mk_specbody (disclose ksb)
-                (fun argh =>
-                   map_or_else (Any.split argh) (fun '(_, argh) => (transl_fun ksb.(ksb_kbody)) argh)
-                               ((transl_fun ksb.(ksb_ubody)) argh))
+                (fun '(mn, argh) =>
+                   my_if (in_dec dec mn frds)
+                         (transl_fun ksb.(ksb_kbody) (mn, argh))
+                         (transl_fun ksb.(ksb_ubody) (mn, argh)))
   .
 
   Definition transl (ms: t): SModSem.t := {|
@@ -942,7 +377,7 @@ Section KTACTICS.
         (at_most: Ord.t) (n1: Ord.t)
         (o: ord)
         r rg (n0: Ord.t) mr_src0 mp_src0 fr_src0
-        mrs_tgt frs_tgt k_src
+        mn mrs_tgt frs_tgt k_src
         (wf: (Σ * Any.t) * (Σ * Any.t) -> Prop)
         (eqr: Σ * Any.t * Σ -> Σ * Any.t * Σ -> Any.t -> Any.t -> Prop)
         stb itr_tgt ctx
@@ -952,13 +387,13 @@ Section KTACTICS.
 
         (POST: gpaco6 (_sim_itree wf) (cpn6 (_sim_itree wf)) rg rg _ _ eqr n1
                        (mr_src0, mp_src0, fr_src0,
-                       (interp_hCallE_tgt stb o (KModSem.transl_itr (_APCK at_most)) ctx) >>= k_src)
+                       (interp_hCallE_tgt stb mn o (KModSem.transl_itr (_APCK at_most)) ctx) >>= k_src)
                       ((mrs_tgt, frs_tgt),
                        itr_tgt))
     :
       gpaco6 (_sim_itree wf) (cpn6 (_sim_itree wf)) r rg _ _ eqr n0
               (mr_src0, mp_src0, fr_src0,
-              (interp_hCallE_tgt stb o (KModSem.transl_itr APCK) ctx) >>= k_src)
+              (interp_hCallE_tgt stb mn o (KModSem.transl_itr APCK) ctx) >>= k_src)
              ((mrs_tgt, frs_tgt),
               itr_tgt).
   Proof.
@@ -974,7 +409,7 @@ Section KTACTICS.
 
         (o: ord)
         r rg (n0: Ord.t) mr_src0 mp_src0 fr_src0
-        mrs_tgt frs_tgt k_src
+        frds mn mrs_tgt frs_tgt k_src
         (at_most: Ord.t)
         (wf: (Σ * Any.t) * (Σ * Any.t) -> Prop)
         (eqr: Σ * Any.t * Σ -> Σ * Any.t * Σ -> Any.t -> Any.t -> Prop)
@@ -982,20 +417,20 @@ Section KTACTICS.
 
         (FUEL: (n1 + 11 < n0)%ord)
         (ftsp: fspec)
-        (FIND: alist_find fn stb = Some (KModSem.disclose ftsp))
+        (FIND: alist_find fn stb = Some (KModSem.disclose frds ftsp))
         (NEXT: (next < at_most)%ord)
 
         (POST: gpaco6 (_sim_itree wf) (cpn6 (_sim_itree wf)) rg rg _ _ eqr n1
                       (mr_src0, mp_src0, fr_src0,
-                       '(ctx1, _) <- (HoareCall true o (KModSem.disclose ftsp) fn (Any.pair tt↑ args) ctx0);;
-                       tau;; tau;; (interp_hCallE_tgt stb o (KModSem.transl_itr (_APCK next)) ctx1)
+                       '(ctx1, _) <- (HoareCall mn true o (KModSem.disclose frds ftsp) fn args ctx0);;
+                       tau;; tau;; (interp_hCallE_tgt mn stb o (KModSem.transl_itr (_APCK next)) ctx1)
                                      >>= k_src)
                       ((mrs_tgt, frs_tgt),
                        itr_tgt))
     :
       gpaco6 (_sim_itree wf) (cpn6 (_sim_itree wf)) r rg _ _ eqr n0
              (mr_src0, mp_src0, fr_src0,
-              (interp_hCallE_tgt stb o (KModSem.transl_itr (_APCK at_most)) ctx0) >>= k_src)
+              (interp_hCallE_tgt mn stb o (KModSem.transl_itr (_APCK at_most)) ctx0) >>= k_src)
              ((mrs_tgt, frs_tgt),
               itr_tgt).
   Proof.
@@ -1025,7 +460,7 @@ Section KTACTICS.
 
         (o: ord)
         r rg (n0: Ord.t) mr_src0 mp_src0 fr_src0
-        mrs_tgt frs_tgt k_src
+        mn mrs_tgt frs_tgt k_src
         (at_most: Ord.t)
         (wf: (Σ * Any.t) * (Σ * Any.t) -> Prop)
         (eqr: Σ * Any.t * Σ -> Σ * Any.t * Σ -> Any.t -> Any.t -> Prop)
@@ -1040,7 +475,7 @@ Section KTACTICS.
     :
       gpaco6 (_sim_itree wf) (cpn6 (_sim_itree wf)) r rg _ _ eqr n0
               (mr_src0, mp_src0, fr_src0,
-              (interp_hCallE_tgt stb o (KModSem.transl_itr (_APCK at_most)) ctx) >>= k_src)
+              (interp_hCallE_tgt stb mn o (KModSem.transl_itr (_APCK at_most)) ctx) >>= k_src)
              ((mrs_tgt, frs_tgt),
               itr_tgt).
   Proof.
@@ -1054,7 +489,7 @@ Section KTACTICS.
   Lemma trivial_init_clo
         A
         (R_src: A -> Any.t -> Any.t -> iProp) (R_tgt: A -> Any.t -> Any.t -> iProp)
-        fn f_tgt gstb body
+        mn frds fn f_tgt gstb body
         (POST: forall a mp_src mp_tgt mr_src mr_tgt fr_src ctx varg
                       (RTGT: R_tgt a mp_src mp_tgt mr_tgt)
                       (ACC: current_iPropL ctx [("INV", R_src a mp_src mp_tgt)])
@@ -1064,39 +499,25 @@ Section KTACTICS.
                    (fun _ _ => eq)
                    89
                    (((mr_src, mp_src), fr_src),
-                    ((interp_hCallE_tgt gstb ord_top (KModSem.transl_fun body varg) ctx)
-                      >>= (HoareFunRet (fun (_: unit) (reth retl: Any.t) => (⌜reth = retl⌝%I): iProp) tt))
+                    ((interp_hCallE_tgt mn gstb ord_top (KModSem.transl_fun body varg) ctx)
+                      >>= (HoareFunRet (fun (_: string) (_: unit) (reth retl: Any.t) =>
+                                          (⌜reth = retl⌝%I): iProp) mn tt))
                    )
                    (((mr_tgt, mp_tgt), ε), (f_tgt varg))
         )
     :
-      sim_fnsem (mk_wf R_src R_tgt) (fn, fun_to_tgt gstb (mk_kspecbody fspec_trivial body body)) (fn, f_tgt)
+      sim_fnsem (mk_wf R_src R_tgt)
+                (fn, fun_to_tgt mn gstb (KModSem.disclose_ksb frds (mk_kspecbody fspec_trivial body body)))
+                (fn, f_tgt)
   .
   Proof.
     init. harg. rename a into aa.
-    Ltac dull_tac :=
-      match goal with
-      | ord_cur: ord |- _ =>
-        assert(ord_cur = ord_top) by (on_current ltac:(fun ACC => clear - ACC); mClear "INV";
-                                      des_ifs; mDesAll; des; ss);
-        subst
-      end;
-      match goal with
-      | |- context[map_or_else (Any.split ?v) ?l (KModSem.transl_fun ?body ?varg_src)] =>
-        let r := constr:(KModSem.transl_fun body varg_src) in
-        let varg := match goal with | [H: context[varg_src = ?varg] |- _] => varg end in
-        replace (map_or_else (Any.split v) l r) with (KModSem.transl_fun body varg);
-        [|on_current ltac:(fun ACC => clear - ACC); mClear "INV"; des_ifs; mDesAll; ss; des; subst; ss; fail]
-      end;
-      mClear "PRE"; rename x into _unused.
-    dull_tac.
-    exploit POST; et. intro SIM.
-    match goal with
-    | [SIM: gpaco6 _ _ _ _ _ _ _ _ ?i0 _ |- gpaco6 _ _ _ _ _ _ _ _ ?i1 _] =>
-      replace i1 with i0; eauto
-    end.
-    repeat f_equal. Local Transparent HoareFunRet. unfold HoareFunRet. Local Opaque HoareFunRet.
-    extensionality x. des_ifs. grind. rewrite map_or_else_same. ss.
+    assert(ord_cur = ord_top).
+    { on_current ltac:(fun ACC => clear - ACC); mClear "INV"; des_ifs; mDesAll; des; ss. }
+    subst. rewrite my_if_same.
+    des_ifs; mDesAll; des; subst.
+    - exploit POST; et.
+    - exploit POST; et.
   Qed.
 
 End KTACTICS.
@@ -1140,13 +561,13 @@ Section KMOD.
   }
   .
 
-  Definition transl (md: t): SMod.t := {|
-    SMod.get_modsem := fun skenv => KModSem.transl (md.(get_modsem) skenv);
+  Definition transl (frds: list mname) (md: t): SMod.t := {|
+    SMod.get_modsem := fun skenv => KModSem.transl frds (md.(get_modsem) skenv);
     SMod.sk := md.(sk);
   |}
   .
 
-  Lemma transl_comm: forall md skenv, KModSem.transl (md.(get_modsem) skenv) = (transl md).(SMod.get_modsem) skenv.
+  Lemma transl_comm: forall md frds skenv, KModSem.transl frds (md.(get_modsem) skenv) = (transl frds md).(SMod.get_modsem) skenv.
   Proof. i. refl. Qed.
 
 End KMOD.
